Some definitions

- Center-of-momentum gamma
- Center-of-momentum reduced mass
- Relative velocity in center-ofmomentum frame (not Lorentz invariant)
- Lorentz-invariant relative velocity computed in the center-of-momentum frame

$$\gamma_C = \frac{E}{E_C} = \frac{m_1 \gamma_1 + m_2 \gamma_2}{m_1 \gamma_1^* + m_2 \gamma_2^*}$$

$$\mu_R^* = \frac{m_1 \gamma_1^* m_2 \gamma_2^*}{m_1 \gamma_1^* + m_2 \gamma_2^*},$$

$$v_{\text{rel}}^* = |\mathbf{v}_1^* - \mathbf{v}_2^*| = \frac{p_1^*}{\mu_R^*},$$

$$v_{\text{rel,invar}}^* = \frac{|\mathbf{v}_1^* - \mathbf{v}_2^*|}{1 - \mathbf{v}_1^* \cdot \mathbf{v}_2^*/c^2}$$

$$= v_{\rm rel}^* / \left(1 + \frac{(p_1^*)^2}{m_1 \gamma_1^* m_2 \gamma_2^* c^2} \right)$$

Superscript * referrers to quantities computed in the center-of-momentum frame

Simplification of last two expressions in Eq. 9 of Perez 2012

$$\frac{\gamma_C p_1^*}{m_1 \gamma_1 + m_2 \gamma_2} = \frac{p_1^*}{m_1 \gamma_1^* + m_2 \gamma_2^*} = \frac{p_1^*}{\mu_R^*} \frac{m_1 \gamma_1^* m_2 \gamma_2^*}{(m_1 \gamma_1^* + m_2 \gamma_2^*)^2},$$

$$\left(\frac{m_1 \gamma_1^* m_2 \gamma_2^*}{(p_1^*)^2} c^2 + 1\right)^2 = \frac{(m_1 \gamma_1^* m_2 \gamma_2^*)^2}{(p_1^*)^4} c^4 \left(1 + \frac{(p_1^*)^2}{m_1 \gamma_1^* m_2 \gamma_2^* c^2}\right)^2$$

$$\Rightarrow \frac{\gamma_C p_1^*}{m_1 \gamma_1 + m_2 \gamma_2} \times \left(\frac{m_1 \gamma_1^* m_2 \gamma_2^*}{(p_1^*)^2} c^2 + 1\right)^2 = \frac{p_1^*}{\mu_R^*} \frac{m_1 \gamma_1^* m_2 \gamma_2^* (\mu_R^*)^2}{(p_1^*)^4} c^4 \left(1 + \frac{(p_1^*)^2}{m_1 \gamma_1^* m_2 \gamma_2^* c^2}\right)^2$$

$$= v_{\text{rel}}^* \frac{m_1 \gamma_1^* m_2 \gamma_2^* c^4}{\left(\mu_R^* v_{\text{rel}}^* v_{\text{rel,invar}}^*\right)^2}$$

Eq. 9 of Perez is same as expression used for s12 in Coulomb collision method

Eq. 9 of Perez

$$\begin{split} s_{12} &= \frac{(q_1q_2)^2 \ln \Lambda}{4\pi\epsilon_0^2 c^4 m_1 \gamma_1 m_2 \gamma_2} \frac{\gamma_C p_1^*}{m_1 \gamma_1 + m_2 \gamma_2} \times \left(\frac{m_1 \gamma_1^* m_2 \gamma_2^*}{(p_1^*)^2} c^2 + 1 \right)^2 n_{12} \Delta t \\ &= \frac{(q_1q_2)^2 \ln \Lambda}{4\pi\epsilon_0^2 c^4 m_1 \gamma_1 m_2 \gamma_2} v_{\rm rel}^* \frac{m_1 \gamma_1^* m_2 \gamma_2^* c^4}{\left(\mu_R^* v_{\rm rel}^* v_{\rm rel,invar}^*\right)^2} n_{12} \Delta t \\ &= \pi \left(\frac{q_1q_2}{2\pi\epsilon_0 \mu_R^* v_{\rm rel}^* v_{\rm rel,invar}^*} \right)^2 \ln \Lambda v_{\rm rel}^* \frac{\gamma_1^* \gamma_2^*}{\gamma_1 \gamma_2} n_{12} \Delta t \\ &= \pi b_0^2 \ln \Lambda v_{\rm rel}^* \frac{\gamma_1^* \gamma_2^*}{\gamma_1 \gamma_2} n_{12} \Delta t \\ &= \pi b_0^2 \ln \Lambda v_{\rm rel}^* \frac{\gamma_1^* \gamma_2^*}{\gamma_1 \gamma_2} n_{12} \Delta t \\ &= \pi b_0^2 \ln \Lambda v_{\rm rel}^* \frac{\gamma_1^* \gamma_2^*}{\gamma_1 \gamma_2} n_{12} \Delta t \\ &= \pi b_0^2 \ln \Lambda v_{\rm rel}^* \frac{\gamma_1^* \gamma_2^*}{\gamma_1 \gamma_2} n_{12} \Delta t \\ &= \pi b_0^2 \ln \Lambda v_{\rm rel}^* \frac{\gamma_1^* \gamma_2^*}{\gamma_1 \gamma_2} n_{12} \Delta t \\ &= \pi b_0^2 \ln \Lambda v_{\rm rel}^* \frac{\gamma_1^* \gamma_2^*}{\gamma_1 \gamma_2} n_{12} \Delta t \\ &= \pi b_0^2 \ln \Lambda v_{\rm rel}^* \frac{\gamma_1^* \gamma_2^*}{\gamma_1 \gamma_2} n_{12} \Delta t \\ &= \pi b_0^2 \ln \Lambda v_{\rm rel}^* \frac{\gamma_1^* \gamma_2^*}{\gamma_1 \gamma_2} n_{12} \Delta t \\ &= \pi b_0^2 \ln \Lambda v_{\rm rel}^* \frac{\gamma_1^* \gamma_2^*}{\gamma_1 \gamma_2} n_{12} \Delta t \\ &= \pi b_0^2 \ln \Lambda v_{\rm rel}^* \frac{\gamma_1^* \gamma_2^*}{\gamma_1 \gamma_2} n_{12} \Delta t \\ &= \pi b_0^2 \ln \Lambda v_{\rm rel}^* \frac{\gamma_1^* \gamma_2^*}{\gamma_1 \gamma_2} n_{12} \Delta t \\ &= \pi b_0^2 \ln \Lambda v_{\rm rel}^* \frac{\gamma_1^* \gamma_2^*}{\gamma_1 \gamma_2} n_{12} \Delta t \\ &= \pi b_0^2 \ln \Lambda v_{\rm rel}^* \frac{\gamma_1^* \gamma_2^*}{\gamma_1 \gamma_2} n_{12} \Delta t \\ &= \pi b_0^2 \ln \Lambda v_{\rm rel}^* \frac{\gamma_1^* \gamma_2^*}{\gamma_1 \gamma_2} n_{12} \Delta t \\ &= \pi b_0^2 \ln \Lambda v_{\rm rel}^* \frac{\gamma_1^* \gamma_2^*}{\gamma_1 \gamma_2} n_{12} \Delta t \\ &= \pi b_0^2 \ln \Lambda v_{\rm rel}^* \frac{\gamma_1^* \gamma_2^*}{\gamma_1 \gamma_2} n_{12} \Delta t \\ &= \pi b_0^2 \ln \Lambda v_{\rm rel}^* \frac{\gamma_1^* \gamma_2^*}{\gamma_1 \gamma_2} n_{12} \Delta t \\ &= \pi b_0^2 \ln \Lambda v_{\rm rel}^* \frac{\gamma_1^* \gamma_2^*}{\gamma_1 \gamma_2} n_{12} \Delta t \\ &= \pi b_0^2 \ln \Lambda v_{\rm rel}^* \frac{\gamma_1^* \gamma_2^*}{\gamma_1 \gamma_2} n_{12} \Delta t \\ &= \pi b_0^2 \ln \Lambda v_{\rm rel}^* \frac{\gamma_1^* \gamma_2^*}{\gamma_1 \gamma_2} n_{12} \Delta t \\ &= \pi b_0^2 \ln \Lambda v_{\rm rel}^* \frac{\gamma_1^* \gamma_2^*}{\gamma_1 \gamma_2} n_{12} \Delta t \\ &= \pi b_0^2 \ln \Lambda v_{\rm rel}^* \frac{\gamma_1^* \gamma_2^*}{\gamma_1 \gamma_2} n_{12} \Delta t \\ &= \pi b_0^2 \ln \Lambda v_{\rm rel}^* \frac{\gamma_1^* \gamma_2^*}{\gamma_1 \gamma_2} n_{12} \Delta t \\ &= \pi b_0^2 \ln \Lambda v_{\rm rel}^* \frac{\gamma_1^* \gamma_2^*}{\gamma_1 \gamma_2} n_{12} \Delta t \\ &= \pi b_0^2 \ln \Lambda v_{\rm rel}^* \frac{\gamma_1^* \gamma_2^*}{\gamma_1 \gamma_2} n_{12} \Delta t \\ &= \pi b_0^2 \ln \Lambda v_{\rm rel}$$